pushback done

dev2016/fsub.v
@@ -227,7 +227,7 @@ Inductive stp2: bool (* whether the last rule may not be transitivity *) ->
 | stp2_sel1: forall G1 G2 GX TX x T2 GH n1,
     indexr x G1 = Some (vty GX TX) ->
     closed 0 0 (length GX) TX ->
-    stp2 false GX TX G2 T2 GH n1 ->
+    stp2 true GX TX G2 T2 GH n1 ->
     stp2 true G1 (TVarF x) G2 T2 GH (S n1)
 | stp2_sel2: forall G1 G2 GX TX x T1 GH n1,
     indexr x G2 = Some (vty GX TX) ->
@@ -1562,7 +1562,7 @@ Proof. intros. repeat eu. eauto. Qed.
 Lemma stpd2_sel1: forall G1 G2 GX TX x T2 GH,
     indexr x G1 = Some (vty GX TX) ->
     closed 0 0 (length GX) TX ->
-    stpd2 false GX TX G2 T2 GH ->
+    stpd2 true GX TX G2 T2 GH ->
     stpd2 true G1 (TVarF x) G2 T2 GH.
 Proof. intros. repeat eu. eauto. Qed.
 Lemma stpd2_sel2: forall G1 G2 GX TX x T1 GH,
@@ -1620,11 +1620,156 @@ Lemma stpd2_trans: forall G1 G2 G3 T1 T2 T3 H,
   stpd2 false G1 T1 G3 T3 H.
 Proof. intros. repeat eu. eapply stpd2_trans_aux; eauto. Qed.
 
+Lemma stp2_narrow_aux: forall n, forall m G1 T1 G2 T2 GH n0,
+  stp2 m G1 T1 G2 T2 GH n0 ->
+  n0 <= n ->
+  forall GH1 GH0 GH' GX1 TX1 GX2 TX2,
+    GH=GH1++[(GX2,TX2)]++GH0 ->
+    GH'=GH1++[(GX1,TX1)]++GH0 ->
+    stpd2 false GX1 TX1 GX2 TX2 GH0 ->
+    stpd2 m G1 T1 G2 T2 GH'.
+Proof.
+  intros n.
+  induction n.
+  - Case "z". intros. inversion H0. subst. inversion H; eauto.
+  - Case "s n". intros m G1 T1 G2 T2 GH n0 H NE. inversion H; subst;
+    intros GH1 GH0 GH' GX1 TX1 GX2 TX2 EGH EGH' HX; eauto.
+    + SCase "top". eapply stpd2_top.
+      subst. rewrite app_length. simpl. rewrite app_length in H0. simpl in H0. apply H0.
+    + SCase "fun". eapply stpd2_fun.
+      eapply IHn; try eassumption. omega.
+      eapply IHn; try eassumption. omega.
+    + SCase "mem". eapply stpd2_mem.
+      eapply IHn; try eassumption. omega.
+    + SCase "sel1". eapply stpd2_sel1; try eassumption.
+      eapply IHn; try eassumption. omega.
+    + SCase "sel2". eapply stpd2_sel2; try eassumption.
+      eapply IHn; try eassumption. omega.
+    + SCase "sela1".
+      unfold id,venv,aenv in *.
+      case_eq (beq_nat x (length GH0)); intros E.
+      * assert (indexr x ([(GX2, TX2)]++GH0) = Some (GX2, TX2)) as A2. {
+          simpl. rewrite E. reflexivity.
+        }
+        assert (indexr x GH = Some (GX2, TX2)) as A2'. {
+          rewrite EGH. eapply indexr_extend_mult. apply A2.
+        }
+        unfold venv in A2'. rewrite A2' in H0. inversion H0. subst.
+        inversion HX as [nx HX'].
+        eapply stpd2_sela1.
+        eapply indexr_extend_mult. simpl. rewrite E. reflexivity.
+        apply beq_nat_true in E. rewrite E. eapply stp2_closed1. eassumption.
+        eapply stpd2_trans.
+        eexists. eapply stp2_extendH_mult. eapply stp2_extendH_mult. eassumption.
+        eapply IHn; try eassumption. omega.
+        reflexivity. reflexivity.
+      * assert (indexr x GH' = Some (GX, TX)) as A. {
+          subst.
+          eapply indexr_same. apply E. eassumption.
+        }
+        eapply stpd2_sela1. eapply A. assumption.
+        eapply IHn; try eassumption. omega.
+    + SCase "selax".
+      unfold id,venv,aenv in *.
+      case_eq (beq_nat x (length GH0)); intros E.
+      * assert (indexr x ([(GX2, TX2)]++GH0) = Some (GX2, TX2)) as A2. {
+          simpl. rewrite E. reflexivity.
+        }
+        assert (indexr x GH = Some (GX2, TX2)) as A2'. {
+          rewrite EGH. eapply indexr_extend_mult. apply A2.
+        }
+        unfold venv in A2'. rewrite A2' in H0. inversion H0. subst.
+        inversion HX as [nx HX'].
+        eapply stpd2_selax.
+        eapply indexr_extend_mult. simpl. unfold id,venv,aenv in *. rewrite E.
+        reflexivity.
+      * assert (indexr x GH' = Some v) as A. {
+          subst.
+          eapply indexr_same. apply E. eassumption.
+        }
+        eapply stpd2_selax. eapply A.
+    + SCase "all".
+      assert (length GH = length GH') as A. {
+        subst. clear.
+        induction GH1.
+        - simpl. reflexivity.
+        - simpl. simpl in IHGH1. rewrite IHGH1. reflexivity.
+      }
+      eapply stpd2_all.
+      eapply IHn; try eassumption. omega.
+      rewrite <- A. reflexivity.
+      rewrite <- A. assumption. rewrite <- A. assumption.
+      subst.
+      eapply IHn with (GH1:=(G2, T4) :: GH1); try eassumption. omega.
+      simpl. reflexivity. simpl. reflexivity.
+    + SCase "wrapf".
+      eapply stpd2_wrapf.
+      eapply IHn; try eassumption. omega.
+    + SCase "transf".
+      eapply stpd2_transf.
+      eapply IHn; try eassumption. omega.
+      eapply IHn; try eassumption. omega.
+Grab Existential Variables. apply 0.
+Qed.
+
+Lemma stpd2_narrow: forall G1 G2 G3 G4 T1 T2 T3 T4 H,
+  stpd2 false G1 T1 G2 T2 H -> (* careful about H! *)
+  stpd2 false G3 T3 G4 T4 ((G2,T2)::H) ->
+  stpd2 false G3 T3 G4 T4 ((G1,T1)::H).
+Proof.
+  intros. inversion H1 as [n H'].
+  eapply (stp2_narrow_aux n) with (GH1:=[]) (GH0:=H). eapply H'. omega.
+  simpl. reflexivity. reflexivity.
+  assumption.
+Qed.
+
+Ltac indexr_contra :=
+  match goal with
+    | H: indexr ?N [] = Some ?V |- _ => simpl in H; inversion H
+  end.
+
+Lemma stpd2_untrans_aux: forall n, forall m G1 G2 G3 T1 T2 T3 n1,
+  stp2 m G1 T1 G2 T2 nil n1 -> n1 < n ->
+  stpd2 true G2 T2 G3 T3 nil ->
+  stpd2 true G1 T1 G3 T3 nil.
+Proof.
+  intros n. induction n; intros; try omega. eu.
+  inversion H; subst;
+  try solve [inversion H1; eexists; eauto];
+  try solve [eapply stpd2_sel1; eauto; eapply IHn; eauto; try omega];
+  try solve [eapply IHn; [eapply H2 | omega | eauto]]; (* wrapf *)
+  try solve [eapply IHn; [eapply H2 | omega | (eapply IHn; [ eapply H3 | omega | eauto ])]]; (* transf *)
+  inversion H1; subst;
+  try solve [eapply stpd2_top; eauto using stp2_closed1];
+  try solve [eapply stpd2_sel2; eauto];
+  try solve [eapply stpd2_fun; eapply stpd2_trans; eauto];
+  try solve [eapply stpd2_mem; eauto; eapply stpd2_trans; eauto];
+  try solve [eapply stpd2_sela1; eauto; eapply stpd2_wrapf; eapply IHn; eauto; try omega];
+  try solve [indexr_contra].
+  - Case "sel2 - sel1".
+    rewrite H6 in H2. inversion H2. subst.
+    eapply IHn. eapply H4. omega. eexists. eassumption.
+  - Case "sel2 - selx".
+    rewrite H6 in H2. inversion H2. subst.
+    eapply stpd2_sel2; eauto.
+  - Case "selx - sel1".
+    rewrite H5 in H3. inversion H3. subst.
+    eapply stpd2_sel1; eauto.
+  - Case "selx - selx".
+    rewrite H5 in H3. inversion H3. subst.
+    eapply stpd2_selx; eauto.
+  - Case "all - all".
+    eapply stpd2_all; eauto.
+    eapply stpd2_trans; eauto.
+    eapply stpd2_trans. eapply stpd2_narrow. eexists. eapply H8. eauto. eauto.
+Grab Existential Variables. apply 0.
+Qed.
+
 Lemma stpd2_untrans: forall G1 G2 G3 T1 T2 T3,
-  stpd2 true G1 T1 G2 T2 [] ->
-  stpd2 true G2 T2 G3 T3 [] ->
-  stpd2 true G1 T1 G3 T3 [].
-Proof. admit. Qed.
+  stpd2 true G1 T1 G2 T2 nil ->
+  stpd2 true G2 T2 G3 T3 nil ->
+  stpd2 true G1 T1 G3 T3 nil.
+Proof. intros. repeat eu. eapply stpd2_untrans_aux; eauto. Qed.
 
 Lemma stpd2_upgrade: forall G1 G2 T1 T2,
   stpd2 false G1 T1 G2 T2 [] ->
